Victor and I just demonstrated that the new definition is equivalent to the old...

src/Fresh_Start.thy
@@ -16,14 +16,14 @@ fun insert_body :: "('id::{linorder}, 'v) elt list \<Rightarrow> ('id, 'v) elt \
         e#x#xs
       else x#insert_body xs e)"
 
-fun insert_after :: "('id::{linorder}, 'v) elt list \<Rightarrow> ('id, 'v) elt \<Rightarrow> 'id option \<rightharpoonup> ('id, 'v) elt list" where
-  "insert_after xs     e None     = Some (insert_body xs e)" |
-  "insert_after []     e (Some i) = None" |
-  "insert_after (x#xs) e (Some i) =
+fun insert :: "('id::{linorder}, 'v) elt list \<Rightarrow> ('id, 'v) elt \<Rightarrow> 'id option \<rightharpoonup> ('id, 'v) elt list" where
+  "insert xs     e None     = Some (insert_body xs e)" |
+  "insert []     e (Some i) = None" |
+  "insert (x#xs) e (Some i) =
      (if fst x = i then
         Some (x#insert_body xs e)
       else
-        do { t \<leftarrow> insert_after xs e (Some i)
+        do { t \<leftarrow> insert xs e (Some i)
            ; Some (x#t)
            })"
 
@@ -38,9 +38,9 @@ using assms
       apply force+
 done
 
-lemma insert_after_insert_body:
+lemma insert_insert_body:
   assumes "distinct (map fst (e1#e2#xs))" "i2 \<noteq> Some (fst e1)"
-  shows   "insert_after (insert_body xs e1) e2 i2 = do { ys \<leftarrow> insert_after xs e2 i2; Some (insert_body ys e1) }"
+  shows   "insert (insert_body xs e1) e2 i2 = do { ys \<leftarrow> insert xs e2 i2; Some (insert_body ys e1) }"
 using assms
   apply(induction xs)
     apply(case_tac "i2")
@@ -64,18 +64,18 @@ using assms
           apply(force simp add: insert_body_commutes)
   done
 
-lemma insert_after_Nil_None:
+lemma insert_Nil_None:
   assumes "fst e1 \<noteq> fst e2" "i \<noteq> fst e2" "i2 \<noteq> Some (fst e1)"
-  shows "insert_after [] e2 i2 \<bind> (\<lambda>ys. insert_after ys e1 (Some i)) = None"
+  shows "insert [] e2 i2 \<bind> (\<lambda>ys. insert ys e1 (Some i)) = None"
 using assms by (case_tac "i2") clarsimp+
 
-lemma insert_after_insert_body_commute:
+lemma insert_insert_body_commute:
   assumes "a \<noteq> aa"
           "aa \<noteq> fst e2"
           "aa \<notin> fst ` set xs"
           "fst e2 \<notin> fst ` set xs"
           "distinct (map fst xs)"
-  shows   "insert_after (insert_body xs (aa, ba)) e2 (Some a) = insert_after xs e2 (Some a) \<bind> (\<lambda>y. Some (insert_body y (aa, ba)))"
+  shows   "insert (insert_body xs (aa, ba)) e2 (Some a) = insert xs e2 (Some a) \<bind> (\<lambda>y. Some (insert_body y (aa, ba)))"
 using assms
   apply(induction xs)
     apply clarsimp
@@ -83,20 +83,20 @@ using assms
     apply(force simp add: insert_body_commutes)
   done
 
-lemma insert_after_commutes:
+lemma insert_commutes:
   assumes "distinct (map fst (e1#e2#xs))" "i1 = None \<or> i1 \<noteq> Some (fst e2)" "i2 = None \<or> i2 \<noteq> Some (fst e1)"
-  shows   "do { ys \<leftarrow> insert_after xs e1 i1; insert_after ys e2 i2 } = do { ys \<leftarrow> insert_after xs e2 i2; insert_after ys e1 i1 }"
+  shows   "do { ys \<leftarrow> insert xs e1 i1; insert ys e2 i2 } = do { ys \<leftarrow> insert xs e2 i2; insert ys e1 i1 }"
 using assms
-  apply(induction rule: insert_after.induct)
+  apply(induction rule: insert.induct)
     apply clarsimp
     apply(erule disjE)
       apply clarsimp
       apply(force simp add: insert_body_commutes)
-      apply(rule insert_after_insert_body, simp, simp, simp)
+      apply(rule insert_insert_body, simp, simp, simp)
     apply(erule disjE)
       apply simp
       apply clarsimp
-      apply(rule insert_after_Nil_None[symmetric], simp, simp, simp)
+      apply(rule insert_Nil_None[symmetric], simp, simp, simp)
     apply(erule disjE)
       apply clarsimp
       apply clarsimp
@@ -110,10 +110,10 @@ using assms
         apply clarsimp
         apply(force simp add: insert_body_commutes)
         apply clarsimp
-        apply(force simp add: insert_after_insert_body_commute)
+        apply(force simp add: insert_insert_body_commute)
         apply clarsimp
         apply(case_tac i2)
-          apply(force cong: Option.bind_cong simp add: insert_after_insert_body)
+          apply(force cong: Option.bind_cong simp add: insert_insert_body)
           apply clarsimp
           apply(case_tac "ab = i")
             apply clarsimp
@@ -121,387 +121,62 @@ using assms
             apply clarsimp
             apply(case_tac "a = ab")
               apply clarsimp
-              apply(force cong: Option.bind_cong simp add: insert_after_insert_body)
+              apply(force cong: Option.bind_cong simp add: insert_insert_body)
               apply clarsimp
               apply(metis bind_assoc)
   done
 
-
-
-
-
-
-
-
-
-
-
-
-
-
-
-
-
-
-
-
-fun insert :: "('id::{linorder}, 'v) elt list \<Rightarrow> ('id, 'v) elt \<Rightarrow> 'id option \<rightharpoonup> ('id::{linorder}, 'v) elt list" where
-  "insert [] e     None     = Some [e]" |
-  "insert [] e     (Some i) = None" |
-  "insert (x#xs) e None     =
+fun insert' :: "('id::{linorder}, 'v) elt list \<Rightarrow> ('id, 'v) elt \<Rightarrow> 'id option \<rightharpoonup> ('id::{linorder}, 'v) elt list" where
+  "insert' [] e     None     = Some [e]" |
+  "insert' [] e     (Some i) = None" |
+  "insert' (x#xs) e None     =
      (if fst x < fst e then
         Some (e#x#xs)
       else
-        case insert xs e None of
+        case insert' xs e None of
           None   \<Rightarrow> None
         | Some t \<Rightarrow> Some (x#t))" |
-  "insert (x#xs) e (Some i) =
+  "insert' (x#xs) e (Some i) =
      (if fst x = i then
-        case insert xs e None of
+        case insert' xs e None of
           None   \<Rightarrow> None
         | Some t \<Rightarrow> Some (x#t)
       else
-        case insert xs e (Some i) of
+        case insert' xs e (Some i) of
           None   \<Rightarrow> None
         | Some t \<Rightarrow> Some (x#t))"
 
-lemma insert_None_condition2 [elim!, dest]:
-  assumes "insert xs e None = None"
+lemma insert'_None_condition2 [elim!, dest]:
+  assumes "insert' xs e None = None"
   shows   "False"
 using assms
-  by (induction xs, auto, case_tac "a < fst e"; clarsimp) (case_tac "insert xsa e None"; clarsimp)
+  by (induction xs, auto, case_tac "a < fst e"; clarsimp) (case_tac "insert' xsa e None"; clarsimp)
 
-lemma insert_Some_empty [elim!, dest]:
-  assumes "insert xs e i = Some []"
-  shows   "False"
-using assms
-  apply (induct xs)
-  apply (case_tac i)
-    apply force
-    apply force
-  apply (case_tac i)
-    apply clarsimp
-    apply (case_tac "a < fst e")
-      apply force
-    apply clarsimp
-    apply (case_tac "insert xs e None")
-      apply force
-    apply force
-  apply clarsimp
-  apply (case_tac "a=aa")
-    apply clarsimp
-    apply (case_tac "insert xs e None")
-      apply force
-    apply force
-  apply clarsimp
-  apply (case_tac "insert xs e (Some aa)")
-    apply force
-  apply force
-done
-
-lemma insert_Some_None_iff:
-  shows   "insert xs e (Some i) = None \<longleftrightarrow> i \<notin> set (map fst xs)"
-  apply(induction xs, simp)
-  apply(case_tac a)
-  apply clarsimp
-  apply(case_tac "aa = i")
-    apply clarsimp
-    apply(case_tac "insert xs e None")
-      apply clarsimp
-      apply clarsimp
-    apply clarsimp
-    apply(case_tac "insert xs e (Some i)")
-      apply force
-      apply clarsimp
-done
-
-lemma insertNoneNoneNoneNone:
-  assumes
-    "distinct (map fst (e1#e2#xs))"
-    "insert xs e1 None = Some xs1"
-    "insert xs e2 None = Some xs2"
-    "insert xs1 e2 None = Some xs1'"
-    "insert xs2 e1 None = Some xs2'"
-  shows "xs1' = xs2'"
-using assms
-  apply (induct xs arbitrary: xs1 xs2 xs1' xs2')
-  apply clarsimp
-  apply(cases "fst e1 < fst e2"; clarsimp)
-    apply(cases "fst e2 < fst e1"; clarsimp)    
-    apply force
-  apply(cases "fst e2 < fst e1")
-    apply force
-  apply force
-  apply clarsimp
-  apply (rename_tac i e xs xs1 xs2 xs1' xs2')
-  apply (case_tac " insert xs e1 None")
-    apply force
-  apply (case_tac " insert xs e2 None")
-    apply force
-  apply (case_tac "i < fst e1")
-   apply (case_tac "fst e1 < fst e2")
-    apply (case_tac "i < fst e2")
-      apply (case_tac "fst e2 < fst e1")
-        using less_trans apply fastforce
-      apply fastforce
-    apply fastforce
-  apply (case_tac "i < fst e2")
-    apply (case_tac "fst e2 < fst e1")
-      apply fastforce
-    apply fastforce
-    apply fastforce
-  apply (case_tac "i < fst e2")
-    apply (case_tac "fst e2 < fst e1")
-      apply fastforce
-    apply fastforce
-  apply (case_tac "insert a e2 None")
-    apply fastforce
-  apply (case_tac "insert aa e1 None")
-    apply fastforce
-  apply fastforce
-done
-
-lemma insertSomeSome1:
-      "insert xs e1 (Some i1') \<bind> (\<lambda>ys. insert ys e2 i2) = insert xs e2 i2 \<bind> (\<lambda>ys. insert ys e1 (Some i1')) \<Longrightarrow>
-       i1' \<noteq> fst e2 \<Longrightarrow>
-       i2 = None \<or> i2 \<noteq> Some (fst e1) \<Longrightarrow>
-       fst e1 \<noteq> fst e2 \<Longrightarrow>
-       fst e1 \<noteq> idx \<Longrightarrow>
-       fst e1 \<notin> fst ` set xs \<Longrightarrow>
-       fst e2 \<noteq> idx \<Longrightarrow>
-       fst e2 \<notin> fst ` set xs \<Longrightarrow>
-       idx \<notin> fst ` set xs \<Longrightarrow>
-       distinct (map fst xs) \<Longrightarrow>
-       i1 = Some i1' \<Longrightarrow>
-       i2 = Some i2' \<Longrightarrow>
-       idx = i1' \<Longrightarrow> (case insert xs e1 None of None \<Rightarrow> None | Some t \<Rightarrow> Some ((idx, e) # t)) \<bind> (\<lambda>ys. insert ys e2 i2) = insert ((i1', e) # xs) e2 i2 \<bind> (\<lambda>ys. insert ys e1 (Some i1'))"
-sorry
-
-lemma insertSomeSome2:
-       "insert xs e1 (Some i1') \<bind> (\<lambda>ys. insert ys e2 i2) = insert xs e2 i2 \<bind> (\<lambda>ys. insert ys e1 (Some i1')) \<Longrightarrow>
-       i1' \<noteq> fst e2 \<Longrightarrow>
-       i2 = None \<or> i2 \<noteq> Some (fst e1) \<Longrightarrow>
-       fst e1 \<noteq> fst e2 \<Longrightarrow>
-       fst e1 \<noteq> idx \<Longrightarrow>
-       fst e1 \<notin> fst ` set xs \<Longrightarrow>
-       fst e2 \<noteq> idx \<Longrightarrow>
-       fst e2 \<notin> fst ` set xs \<Longrightarrow>
-       idx \<notin> fst ` set xs \<Longrightarrow>
-       distinct (map fst xs) \<Longrightarrow>
-       i1 = Some i1' \<Longrightarrow>
-       i2 = Some i2' \<Longrightarrow>
-       idx \<noteq> i1' \<Longrightarrow> (case insert xs e1 (Some i1') of None \<Rightarrow> None | Some t \<Rightarrow> Some ((idx, e) # t)) \<bind> (\<lambda>ys. insert ys e2 i2) = insert ((idx, e) # xs) e2 i2 \<bind> (\<lambda>ys. insert ys e1 (Some i1'))"
-sorry
-
-lemma insert_Cons_Some_Some_bind:
-  assumes "i1 \<noteq> fst x" "i2 \<noteq> fst x"
-  shows "insert (x#xs) e1 (Some i1) \<bind> (\<lambda>ys. insert ys e2 (Some i2)) = insert xs e1 (Some i1) \<bind> (\<lambda>ys. insert ys e2 (Some i2) \<bind> (\<lambda>zs. Some (x#zs)))"
-using assms
-  apply clarsimp
-  apply(case_tac "insert xs e1 (Some i1)")
-    apply clarsimp+
-    apply(case_tac "insert a e2 (Some i2)")
+lemma insert_body_insert':
+  shows "insert' list (a, b) None = Some (insert_body list (a, b))"
+  apply(induction list)
     apply clarsimp+
   done
 
-lemma foo:
-  assumes "i1 = fst x" "i2 \<noteq> fst x"
-  shows "insert (x#xs) e1 (Some i1) \<bind> (\<lambda>ys. insert ys e2 (Some i2)) = insert xs e1 None \<bind> (\<lambda>ys. insert ys e2 (Some i2) \<bind> (\<lambda>zs. Some (x#zs)))"
-using assms
-sorry
-
-lemma insert_preserves_fst_set:
-  assumes "i2' \<notin> set (map fst xs)" "insert xs e1 None = Some a" "i2' \<noteq> fst e1"
-  shows   "i2' \<notin> set (map fst a)"
-using assms
-sorry
-
-lemma insert_commutes:
-  assumes "distinct (map fst (e1#e2#xs))" "i1 = None \<or> i1 \<noteq> Some (fst e2)" "i2 = None \<or> i2 \<noteq> Some (fst e1)"
-  shows   "insert xs e1 i1 \<bind> (\<lambda>ys. insert ys e2 i2) = insert xs e2 i2 \<bind> (\<lambda>ys. insert ys e1 i1)"
-using assms
-  apply(induction xs)
-  (* Empty case *)
-  apply clarsimp
-  apply(cases i1; clarsimp; cases i2; clarsimp)
-  apply force
-  (* Step case *)
-  apply clarsimp
-  apply (rename_tac idx e xs)
-  (* i1 = None *)
-  apply(cases i1, clarsimp)
-    (* i2 = None *)
-    apply(cases i2; clarsimp)
-      apply(case_tac "insert xs e1 None")
-        apply force
-      apply(case_tac "insert xs e2 None")
-        apply force
-      apply force
-    (* i2 = Some i *)
-    apply (rename_tac i2')
-    apply(case_tac "insert xs e1 None")
-      (* insert xs e1 None = None *)
-      apply force
-    (* insert xs e1 None = Some xs1 *)
-    apply(rename_tac xs1) 
-    apply(case_tac "insert xs e2 (Some i2')")
-      apply clarsimp
-      apply (case_tac "insert xs e2 None")
-        apply force
-      apply (rename_tac xs2')
-      apply clarsimp
-      apply (case_tac "insert xs1 e2 None")
-        apply force
-      apply (rename_tac xs1')
-      apply clarsimp
-      apply (case_tac "insert xs2' e1 None")
-        apply force
-      apply clarsimp
-      apply(rule insertNoneNoneNoneNone)
-        prefer 2
-        apply assumption
-        prefer 2
-        apply assumption back
-        apply simp
-        apply simp
-        apply simp
-      apply clarsimp
-      apply (case_tac "insert xs e2 None")
-        apply force
-      apply clarsimp
-      apply (case_tac "insert xs1 e2 None")
-        apply force
-      apply clarsimp  
-      apply (case_tac "insert aa e1 None")
-        apply force
-      apply clarsimp
-      apply(rule insertNoneNoneNoneNone)
-        prefer 2
-        apply assumption
-        prefer 2
-        apply assumption back
-        apply simp
-        apply simp
-        apply simp
-  (* i1 = Some i1' *)
-  apply (rename_tac i1')
-  apply(cases i2, clarsimp)
-    (* i2 = None *)
-    apply(case_tac "insert xs e1 None")
-      apply force
-    apply(case_tac "insert xs e2 None")
-      apply force
-    apply(case_tac "insert xs e1 (Some i1')")
-      apply clarsimp
-      apply (case_tac "insert a e2 None")
-        apply force
-      apply clarsimp
-      apply (case_tac "insert aa e1 None")
-        apply force
-      apply clarsimp
-      apply(rule insertNoneNoneNoneNone)
-        prefer 2
-        apply assumption
-        prefer 2
-        apply assumption back
-        apply simp
-        apply simp
-        apply simp
+lemma insert_insert':
+  shows "insert = insert'"
+  apply(rule ext)+
+  apply(induct_tac x)
+    apply(case_tac "xb")
+      apply simp+
     apply clarsimp
-      apply (case_tac "insert a e2 None")
+    apply(case_tac "xb")
+      apply simp
+      apply(rule impI)
+      apply(case_tac "insert' list (a, b) None")
+        apply clarsimp+
+      apply safe
+      apply(case_tac "insert' list (a, b) None")
         apply force
+        apply(force simp add: insert_body_insert')
+    apply(case_tac "insert' list (a, b) (Some ab)")
       apply clarsimp
-      apply (case_tac "insert aa e1 None")
-        apply force
       apply clarsimp
-      apply(rule insertNoneNoneNoneNone)
-        prefer 2
-        apply assumption
-        prefer 2
-        apply assumption back
-        apply simp
-        apply simp
-        apply simp
-
-(* i2 = Some i2' *)
-apply (rename_tac i2')
-  apply clarsimp
-  apply(case_tac "insert xs e1 None")
-    apply force
-  apply clarsimp
-  apply(case_tac "insert xs e2 None")
-    apply force
-  apply clarsimp
-  apply(case_tac "insert a e2 None")
-    apply force
-  apply clarsimp
-  apply(case_tac "insert aa e1 None")
-    apply force
-  apply clarsimp
-  apply(case_tac "i2' = i1'")
-    apply clarsimp
-    apply(case_tac "idx = i1'")
-      apply clarsimp
-      apply(rule insertNoneNoneNoneNone)
-        prefer 2
-        apply assumption
-        prefer 2
-        apply assumption back
-        apply simp
-        apply simp
-        apply simp
-      apply clarsimp
-      apply(case_tac "insert xs e1 (Some i1')")
-        apply clarsimp
-        apply(case_tac "insert xs e2 (Some i1')")
-          apply clarsimp
-          apply clarsimp
-        apply clarsimp
-        apply(case_tac "insert xs e2 (Some i1')")
-          apply clarsimp
-          apply clarsimp
-  apply safe
-    apply clarsimp
-    apply(case_tac "insert xs e2 (Some i2')")
-      apply clarsimp
-        apply(case_tac "insert xs e2 (Some i2')")
-          apply clarsimp
-          apply(subgoal_tac "insert a e2 (Some i2') = None")
-          prefer 2
-          apply(subst (asm) insert_Some_None_iff)
-          apply(subst insert_Some_None_iff)
-
-
-
-          apply(frule insert_Some_NoneE)
-          apply clarsimp
-          apply(case_tac "insert ad e1 None")
-            apply clarsimp
-            apply clarsimp
-    
-(*
-  apply(case_tac "idx \<noteq> i1' \<and> idx \<noteq> i2'")
-  apply(subst insert_Cons_Some_Some_bind, simp)
-  apply(erule conjE, simp, simp)+
-  apply(subgoal_tac "insert xs e2 (Some i2') \<bind> (\<lambda>ys. insert ys e1 (Some i1') \<bind> (\<lambda>zs. Some ((idx, e) # zs))) =
-       (case insert xs e2 (Some i2') of None \<Rightarrow> None | Some t \<Rightarrow> Some ((idx, e) # t)) \<bind> (\<lambda>ys. insert ys e1 (Some i1'))")
-  prefer 2
-  apply clarsimp
-*)
-
-apply clarsimp
-apply (rule conjI, rule impI)
-  (* idx = i1' *)
-  prefer 2
-  apply clarsimp
-  prefer 2
-  apply assumption
-apply (rule insertSomeSome1)
-apply assumption+
-apply (rule impI)
-apply (rule insertSomeSome2)
-apply assumption+
-done
-
+  done
 
 end
